EffectSSA/ProofSketch/VarSet.lean
@@ -1,6 +1,8 @@
 module
 
 import Mathlib.Data.Set.Basic
+import Mathlib.Data.Set.Defs
+import Mathlib.Data.Set.Lattice
 
 /-!
 # VarSet
@@ -13,6 +15,180 @@ public axiom Var : Type
 /-- `VarSet` is a set of variables. -/
 public def VarSet := Set Var
 
+/-!
+For some reason, having the following definitions be computable requires the relevant definitions to
+be exposed, which would require publicly importing Finset from Mathlib.
+We don't want this, and don't actually need to compute with VarSet anyway,
+so we conceed and make everything noncomputable.
+
+The one use-case for which computability would've been nice, is to show decidability of, e.g,
+the membership relation. This is not strictly needed, though.
+
+The error raised when things are computable mentions that it is a compiler limitation that may be
+addressed in the future, rather than a fundamental requirement, at which time we could have
+this be computable.
+-/
+noncomputable section
+
 namespace VarSet
 
+def toSet : VarSet → Set Var := id
+def ofSet : Set Var → VarSet := id
+
+public section
+
+/-! ### Standard Set Operations -/
+
+def Subset (A B : VarSet) := A.toSet ⊆ B.toSet
+instance : HasSubset VarSet where Subset := Subset
+
+def union (A B : VarSet) : VarSet := ofSet <| A.toSet ∪ B.toSet
+instance : Union VarSet where union := union
+
+def inter (A B : VarSet) : VarSet := ofSet <| A.toSet ∩ B.toSet
+instance : Inter VarSet where inter := inter
+
+def empty : VarSet := ofSet ∅
+instance : EmptyCollection VarSet where emptyCollection := empty
+
+def singleton (v : Var) : VarSet := ofSet { v }
+instance : Singleton Var VarSet where singleton := singleton
+
+def Mem (A : VarSet) (v : Var) := v ∈ A.toSet
+instance : Membership Var VarSet where mem := Mem
+
+def sdiff (A B : VarSet) := ofSet <| A.toSet \ B.toSet
+instance : Sub VarSet where sub := sdiff
+-- ^ N.B: we use `-` notation over `\` set difference since the latter is
+--        is defined in Mathlib
+
+section Lemmas
+variable {A B C : VarSet}
+
+/-! ### ext -/
+
+@[simp, grind =] private theorem mem_toSet (x : Var) (A : VarSet) :
+    x ∈ A.toSet ↔ x ∈ A := by rfl
+@[simp, grind =] private theorem mem_ofSet (x : Var) (A : Set Var) :
+    x ∈ (ofSet A) ↔ x ∈ A := by rfl
+
+@[ext]
+theorem ext (h : ∀ x, x ∈ A ↔ x ∈ B) : A = B := by
+  show A.toSet = B.toSet
+  ext x
+  simpa using h x
+
+/-! ### empty -/
+
+@[simp, grind .] theorem not_mem_empty : v ∉ (∅ : VarSet) := by grind
+
+theorem eq_empty_iff : A = ∅ ↔ (∀ v, v ∉ A) := by
+  constructor
+  · rintro rfl; grind
+  · intro h; ext; grind
+
+/-! ### union -/
+
+@[simp, grind =] theorem mem_union : v ∈ A ∪ B ↔ v ∈ A ∨ v ∈ B := by sorry
+
+@[simp, grind =] theorem empty_union : ∅ ∪ A = A := by ext; grind
+@[simp, grind =] theorem union_empty : A ∪ ∅ = A := by ext; grind
+@[simp, grind =] theorem union_self  : A ∪ A = A := by ext; grind
+
+@[grind =] theorem union_assoc : A ∪ B ∪ C = A ∪ (B ∪ C) := by ext; grind
+@[grind =] theorem union_comm : A ∪ B = B ∪ A := by ext; grind
+
+@[simp] theorem union_eq_empty_iff : A ∪ B = ∅ ↔ A = ∅ ∧ B = ∅ := by
+  sorry
+
+/-! ### inter -/
+
+@[simp, grind =] theorem mem_inter : v ∈ A ∩ B ↔ v ∈ A ∧ v ∈ B := by sorry
+
+@[simp, grind =] theorem empty_inter : ∅ ∩ A = ∅ := by ext; grind
+@[simp, grind =] theorem inter_empty : A ∩ ∅ = ∅ := by ext; grind
+@[simp, grind =] theorem inter_self  : A ∩ A = A := by ext; grind
+
+@[grind =] theorem inter_assoc : A ∩ B ∩ C = A ∩ (B ∩ C) := by ext; grind
+@[grind =] theorem inter_comm : A ∩ B = B ∩ A := by ext; grind
+
+@[grind =] theorem union_inter : (A ∪ B) ∩ C = (A ∩ C) ∪ (B ∩ C) := by ext; grind
+@[grind =] theorem inter_union : A ∩ (B ∪ C) = (A ∩ B) ∪ (A ∩ C) := by ext; grind
+
+/-! ### subset -/
+
+@[grind →] theorem mem_of_mem_subset (h : A ⊆ B) : a ∈ A → a ∈ B := by sorry
+
+end Lemmas
+
+/-! ### Disjoint -/
+
+@[expose] def Disjoint (A B : VarSet) : Prop :=
+  A ∩ B = ∅
+
+section Lemmas
+variable {A B : VarSet}
+attribute [local grind] Disjoint
+
+@[simp, grind .] theorem empty_disjoint : Disjoint ∅ A := by grind
+@[simp, grind .] theorem disjoint_empty : Disjoint A ∅ := by grind
+@[simp, grind =] theorem disjoint_self : A.Disjoint A ↔ A = ∅ := by grind
+
+@[simp, grind =] theorem union_disjoint :
+    Disjoint (A ∪ B) C ↔ Disjoint A C ∧ Disjoint B C := by
+  simp [Disjoint, union_inter]
+
+@[simp, grind =] theorem disjoint_union :
+    Disjoint A (B ∪ C) ↔ Disjoint A B ∧ Disjoint A C := by
+  simp [Disjoint, inter_union]
+
+@[grind =] theorem disjoint_symm : A.Disjoint B ↔ B.Disjoint A := by grind
+
+theorem inter_eq_of_disjoint (h : A.Disjoint B) : A ∩ B = ∅ := by grind
+grind_pattern inter_eq_of_disjoint => A.Disjoint B, A ∩ B
+
+theorem disjoint_iff_mem : A.Disjoint B ↔ (∀ x, ¬(x ∈ A ∧ x ∈ B)) := by
+  sorry
+
+@[grind →] theorem not_mem_of_disjoint (h : A.Disjoint B) {x} :
+    x ∈ A → x ∉ B := by
+  sorry
+
+@[grind →, grind <=]
+theorem disjoint_of_supset_disjoint : A ⊆ B → B.Disjoint C → A.Disjoint C := by
+  grind [disjoint_iff_mem]
+
+
+end Lemmas
+
+/-! ### setOf -/
+
+def setOf (P : Var → Prop) : VarSet :=
+  ofSet <| _root_.setOf P
+
+/-! ### Map -/
+
+/--
+Given a function `f : Var → VarSet` and a set `A : VarSet`, return the set
+  `{ f a | a ∈ A }`
+-/
+def flatMap (f : Var → VarSet) (A : VarSet) : VarSet :=
+  ofSet <| ⋃ (a ∈ A), f a
+
+/--
+Given a function `f : α → VarSet` and a list `as : List α`, return the set
+  `{ f a | a ∈ A }`
+-/
+def ofListMap [DecidableEq α] (f : α → VarSet) (as : List α) : VarSet :=
+  ofSet <| ⋃ (a ∈ as), (f a).toSet
+
+section Lemmas
+variable {A : VarSet}
+
+@[simp, grind =] theorem mem_flatMap : x ∈ A.flatMap f ↔ ∃ y ∈ A, x ∈ f y := by
+  simp [flatMap]; rfl
+
+end Lemmas
+
+end
 end VarSet
