EffectSSA/ProofSketch/AxiomCheck.lean
@@ -9,16 +9,20 @@ namespace EffectSSA.ProofSketch
 
 /--
 info: 'EffectSSA.ProofSketch.Pattern.ctxRefine_of_denoteRefine' depends on axioms: [propext,
+ sorryAx,
  Classical.choice,
  Quot.sound,
  Inst,
  State,
  Val,
  Var,
+ Inst.args,
  Inst.denote,
  Inst.denote_isRefinedBy_congr,
+ Inst.results,
  SEnv.refine_refl,
  State.Refine,
+ State.initial,
  Val.Refine]
 -/
 #guard_msgs in #print axioms Pattern.ctxRefine_of_denoteRefine
