EffectSSA/ProofSketch/InstSeq.lean
@@ -1,0 +1,113 @@
+module
+
+public import EffectSSA.ProofSketch.Inst
+public import EffectSSA.ProofSketch.VarSet
+
+/-!
+# Instruction Sequence
+-/
+namespace EffectSSA.ProofSketch
+
+@[expose] public abbrev InstSeq := List Inst
+
+namespace InstSeq
+
+/-!
+## Variables
+-/
+noncomputable section Vars
+
+def argsResults : InstSeq → VarSet × VarSet := go ∅ ∅
+where go (A R : VarSet)
+  | [] => (A, R)
+  | i :: is =>
+    let A := A ∪ (i.args - R)
+    let R := R ∪ i.results
+    go A R is
+
+/--
+`is.args` is the set of free arguments used in sequence `is`.
+
+Note: "free" means that any argument of an instruction `i ∈ is` that is also the
+result of any preceding instructions are *not* included in `is.args`.
+-/
+public def args (is : InstSeq) : VarSet :=
+  is.argsResults.1
+
+/-- `is.results` is the set of all results of sequence `is`. -/
+public def results (is : InstSeq) : VarSet :=
+  is.argsResults.2
+
+section Lemmas
+variable {i : Inst} {is : InstSeq}
+attribute [local grind] results args argsResults argsResults.go
+
+@[grind =] theorem argsResults_go_snd : (argsResults.go A R is).2 = R ∪ is.results := by
+  suffices ∀ A' R',
+    (argsResults.go A (R ∪ R') is).snd = R ∪ (argsResults.go A' R' is).snd
+  by simp [results, argsResults]; grind
+  induction is generalizing A R <;> grind
+
+@[simp, grind =] public theorem results_nil  : results [] = ∅ := by rfl
+@[simp, grind =] public theorem results_cons : results (i :: is) = i.results ∪ is.results := by
+  simp [results, argsResults]; grind
+
+end Lemmas
+
+/-! ### getDef / usesAt  -/
+
+/--
+`is.getDef? v` returns an instruction `i ∈ is` s.t. `v ∈ i.results`,
+or `none` if no such instruction exists
+-/
+public noncomputable def getDef? (v : Var) : (is : InstSeq) → Option { i // i ∈ is ∧ v ∈ is.results }
+  | [] => none
+  | i :: is =>
+      open Classical in
+      if hi : v ∈ i.results then
+        some ⟨i, by grind⟩
+      else
+        (getDef? v is).map (fun ⟨i, hi⟩ => ⟨i, by grind⟩)
+
+/--
+`is.usesAt v` is the set of all transitive arguments that are used to compute
+variable `v`.
+
+That is, if `v` is defined by instruction `i ∈ is`, then `is.usesAt v` is the
+union of `i.args` with the recursive set `{ is.usesAt y | y ∈ i.args }`.
+
+If no instruction of `is` defines the variable `v` as a result,
+then `is.usesAt v` is the empty set.
+-/
+public noncomputable def usesAt (v : Var) : InstSeq → VarSet
+  | [] => ∅
+  | i :: (is : InstSeq) =>
+      open Classical in
+      if v ∈ i.results then
+        i.args ∪ i.args.flatMap (is.usesAt ·)
+      else
+        is.usesAt v
+
+section Lemmas
+variable {is : InstSeq}
+
+@[grind =]
+public theorem mem_usesAt :
+    y ∈ is.usesAt x ↔ ∃ i ∈ is, x ∈ i.results ∧
+      (y ∈ i.args ∨ ∃ z ∈ i.args, y ∈ is.usesAt z) := by
+  induction is generalizing y
+  · grind [usesAt]
+  case cons i is ih =>
+    stop
+    by_cases y ∈ i.results
+    · have : usesAt x (i :: is) = i.args ∪ i.args.flatMap (usesAt · is) := by
+        sorry
+      simp_all
+      grind
+    split
+    · grind
+    · simp_all
+
+end Lemmas
+end Vars
+end InstSeq
